@prefix ah: <http://www.purl.com/ah/vocab/> .
@prefix ah-vocab:<http://www.purl.com/ah/ves/>.
@prefix dct: <http://purl.org/dc/terms/> .
@prefix foaf: <http://xmlns.com/foaf/0.1/> .
@prefix rdfs: <http://www.w3.org/2000/01/rdf-schema#> .
@prefix schema: <http://schema.org/> .
@prefix voaf: <http://labs.mondeca.com/vocab/voaf#> .
@prefix skos: <http://www.w3.org/2004/02/skos/core#> .
@prefix xsd: <http://www.w3.org/2001/XMLSchema#> .
@prefix vann: <http://purl.org/vocab/vann/> .
@prefix dbo:<http://dbpedia.org/ontology/> .
@prefix time:<http://www.w3.org/2006/time#> .
@prefix edm:<http://www.europeana.eu/schemas/edm> .
@prefix crm:<http://www.cidoc-crm.org/cidoc-crm/>
@prefix crmsci:<https://cidoc-crm.org/extensions/crmsci/> .
@prefix crmarchaeo:<http://www.cidoc-crm.org/extensions/crmarchaeo/> .
@prefix geo:<http://www.w3.org/2003/01/geo/wgs84_pos#> .

<http://www.purl.com/ah/vocab/> 	a voaf:metadataVoc, owl:Ontology;
  voaf:specializes ah:;
  dct:title "Asset Description Metadata Schema - ArrowHeads' Metadata Scheme"@en;
  rdfs:label "Asset Description Metadata Schema - ArrowHeads' Metadata Scheme"@en;
	dct:abstract "ArowHeads is a profile of Arrowheads Vocabulary, used to describe semantic assets (or just 'Assets'), defined as highly reusable metadata (e.g. xml schemata, generic data models) and reference data (e.g. code lists, taxonomies, dictionaries, vocabularies) that are used for ..............."@en;
	dct:creator [schema:affiliation <http://www.w3.org/data#W3C>;
	  rdfs:seeAlso ;
  	foaf:homepage ;
  	foaf:name ] ,
    [schema:affiliation [foaf:homepage ; foaf:name ];
  	rdfs:seeAlso ;
	  foaf:homepage ;
	  foaf:name ] ,
    [rdfs:seeAlso ; foaf:homepage ;
    	foaf:name ;
  foaf:maker[foaf:name "XXXXXXXXXXXXXXXXXXXXXXXXX"; foaf:homepage ];
	dct:description """This is the RDF encoding of the data Model for the description of the Chalcolithic and Early/Middle Bronze Age arrowheads .""";
	dct:modified "2024-"^^xsd:date;
	vann:preferredNamespacePrefix "ah";
	vann:preferredNamespaceUri "http://www.purl.com/ah/vocab/";
	rdfs:comment "This file specifies the set of RDF classes and properties used in the ArroWheads MAP"@en;
	wdrs:describedby .


              #======<>===============================<>=====#
#===========  #------<>-------------------------------<>-----#  ===========#
#===========  #------<>       CLASSES                 <>-----#  ===========#
#===========  #------<>-------------------------------<>-----#	===========#
              #======<>===============================<>=====#

ah:Morphology
	a rdfs:Class;
	rdfs:comment "Morphology of the arrowhead."@en;
	rdfs:isDefinedBy <http://www.purl.com/ah/vocab/>;
	rdfs:label "Morphology"@en.

ah:BaseShapeDetails
	a rdfs:Class;
	rdfs:comment "The arrowhead base Details."@en;
	rdfs:isDefinedBy <http://www.purl.com/ah/vocab/>;
	rdfs:label "Arrowhead-Morphology-BaseShapeDetails"@en.

ah:Typometry
  a rdfs:Class;
  rdfs:comment "Topometry of the arrowhead."@en;
  rdfs:isDefinedBy <http://www.purl.com/ah/vocab/>;
  rdfs:label "Typometry"@en.

ah:Chipping
	a rdfs:Class;
	rdfs:comment "Chipping of the arrowhead."@en;
	rdfs:isDefinedBy <http://www.purl.com/ah/vocab/>;
  rdfs:label "ArrowHead - Chipping."@en;
	rdfs:label "Shipping"@en.

              #======<>===============================<>=====#
#===========  #------<>-------------------------------<>-----#  ===========#
#===========  #------<>          Properties           <>-----#  ===========#
#===========  #------<>-------------------------------<>-----#	===========#
              #======<>===============================<>=====#

#>-----------------------------------------<#
#>           Object Properties             <#
#>-----------------------------------------<#


ah:hasGPSCoordinates
	a rdf:Property,	owl:ObjectProperty;
	rdfs:comment "This property records the Gps coordinates of the central point of the excavation's location in degrees ."@en;
	rdfs:isDefinedBy <http://www.purl.com/ah/vocab/>;
	rdfs:label "Location - has GPS Coordinates"@en;
  rdfs:domain crmarchaeo:A9;
	rdfs:range geo:SpatialThing;
	vann:usageNote "Non-mandatory Property - 0..1"@en .

ah:hasResponsible
  a rdf:Property,	owl:ObjectProperty;
  rdfs:comment "This property records the responsible of an instance of Archaeologist."@en;
  rdfs:isDefinedBy <http://www.purl.com/ah/vocab/>;
  rdfs:label "Excavation - has a resposible Archaeologist"@en;
  rdfs:domain crmarchaeo:A9;
  rdfs:range foaf:Person;
  vann:usageNote "non-mandatory Property - 0..1"@en .

  ah:hasContext
  	a rdf:Property,	owl:ObjectProperty;
  	rdfs:comment "This property records the context of an instance of Context."@en;
  	rdfs:isDefinedBy <http://www.purl.com/ah/vocab/>;
  	rdfs:label "Excavation - hasCcontext"@en;
    rdfs:domain crmarchaeo:A9;
  	rdfs:range crmarchaeo:A1;
  	vann:usageNote "non-mandatory Property - 0..M"@en .

ah:hasStratigraphicVolumeUnit;
  	a rdf:Property,	owl:ObjectProperty;
  	rdfs:comment "A context has several StratigraphicVolumeUNit(CIDOC CRM A1)."@en;
  	rdfs:label "A context has several StratigraphicVolumeUNit"@en;
    rdfs:domain crmarchaeo:A1;
  	rdfs:range crmarchaeo:A2;
  	vann:usageNote "non-mandatory Property - 0..M"@en.

ah:hasTimeline
  	a rdfs:Class;
  	rdfs:comment "This property points to the specific timeline of the the layer ."@en;
  	rdfs:isDefinedBy <http://www.purl.com/ah/vocab/>;
  	rdfs:label "StratigraphicVolumeUnit - has a timeline"@en;
    rdfs:domain crmarchaeo:A2;
  	rdfs:range time:TemporalEntity
  	vann:usageNote "non-mandatory Property - o..1"@en .

ah:foundInAStratigraphicVolumeUnit
  a rdf:Property, owl:ObjectProperty;
  rdfs:comment "Points to the instances of the StratigraphicVolumeUnit of the finding."@en;
  rdfs:label "Encounter Event - an arrowhead found in a specific StratigraphicVolumeUnit"@en;
  rdfs:domain crmsci:S19;
  rdfs:range crmarchaeo:A2;
  vann:usageNote "non-mandatory Property - 0..M"@en .

ah:foundInAContext
  a rdf:Property, owl:ObjectProperty;
  rdfs:comment "Points to the instance of the Context of the finding."@en;
  rdfs:label "The Encounter Event - an arrowhead found in a specific Context"@en;
  rdfs:domain crmsci:S19;
  rdfs:range crmarchaeo:A1;
  vann:usageNote "Mandatory Property - 1..1"@en .

ah:arrowheadFindInGPSCoordinates
	a rdf:Property,	owl:ObjectProperty;
	rdfs:comment "This property points to the definition of the GPS coordinates of the location of the arrowhead in the context."@en;
	rdfs:isDefinedBy <http://www.purl.com/ah/vocab/>;
	rdfs:label "ArrowHead - gpslocation"@en;
  rdfs:domain crm:E24;
	rdfs:range geo:SpatialThing;
	vann:usageNote "Non-mandatory Property - 0..1"@en.

ah:hasMorphology
	a rdf:Property,	owl:ObjectProperty;
	rdfs:comment "This property points to an instance of the definition of the morphology of the arrowhead.."@en;
	rdfs:isDefinedBy <http://www.purl.com/ah/vocab/>;
	rdfs:label "ArrowHead - morphology"@en;
  rdfs:domain crm:E24;
	rdfs:range ah:Morphology;
	vann:usageNote "Non-mandatory Property - 0..1"@en.

ah:hasBaseShapeDetails
  	a rdf:Property,	owl:ObjectProperty;
  	rdfs:comment "This property points to an instance with the description of the base details of the arrowhead base."@en;
  	rdfs:isDefinedBy <http://www.purl.com/ah/vocab/>;
  	rdfs:label "ArrowHead - Morphology - hasBaseDetails"@en;
    rdfs:domain ah:Morphology;
  	rdfs:range ah:BaseShapeDetails;
  	vann:usageNote "Non-mandatory Property - 0..1"@en.

ah:hasTypometry
	a rdf:Property,	owl:ObjectProperty;
	dct:identifier "ah:typometry"@en;
	rdfs:comment "This property points to an instance of the definition of the typometry of the Arrowhead."@en;
	rdfs:isDefinedBy <http://www.purl.com/ah/vocab/>;
	rdfs:label "ArrowHead - typometry"@en;
  rdfs:domain crm:E24;
	rdfs:range ah:Typometry;
	vann:usageNote "Non-mandatory Property - 0..1"@en.

ah:hasChipping
  a rdf:Property,	owl:ObjectProperty;
  rdfs:comment "This Property points to an instance of the definition of the chipping of the arrowhead.."@en;
  rdfs:isDefinedBy <http://www.purl.com/ah/vocab/>;
  rdfs:label "ArrowHead - has chipping"@en;
  rdfs:domain crm:E24;
  rdfs:range ah:Chipping;
  vann:usageNote "Non mandatory Property - 0..1"@en.

#>-----------------------------------------<#
#>           Data Properties             <#
#>-----------------------------------------<#

ah:shape
	a rdf:Property,	owl:DataProperty;
	rdfs:comment "This property records the shape of the arrowhead. A good practice is to use the controlled vocabulary for AH-Shape."@en;
	rdfs:isDefinedBy <http://www.purl.com/ah/vocab/>;
	rdfs:label "ArrowHead - shape"@en;
  rdfs:domain crm:E24;
	rdfs:range ah-vocab:AH-Shape;
	vann:usageNote "Non-mandatory Property - 0..1"@en.

ah:variant
  	a rdf:Property,	owl:DataProperty;
  	rdfs:comment "Thickness index. A good practice is to use the Controlled Vocabulary XX."@en;
  	rdfs:isDefinedBy <http://www.purl.com/ah/vocab/>;
  	rdfs:label "ArrowHead - arrowHeadVariant"@en;
    rdfs:domain crm:E24;
  	rdfs:range ah-vocab:AH-Variant;
  	vann:usageNote "Optional Property - 0..1"@en.

ah:point
	a rdf:Property,	owl:DataProperty;
	rdfs:comment "Definition of the tip of the arrowhead. A good practice is to use the contreolled vocabulary AH-Point."@en;
	rdfs:isDefinedBy <http://purl.org/dc/terms/>;
	rdfs:label "Arrowhead-Morphology - point"@en;
  rdfs:domain ah:Morphology;
	rdfs:range ah-vocab:AH-Point;
	vann:usageNote "Non-mandatory Property - 0..1"@en .

ah:body
	a rdf:Property,	owl:DataProperty;
  rdfs:comment "Does the arrowhead presents symmetry?"@en;
	rdfs:isDefinedBy <http://www.purl.com/ah/vocab/>;
	rdfs:label "Arrowhead-Morphology - body"@en;
  rdfs:domain ah:Morphology;
	rdfs:range xsd:boolean;
	vann:usageNote "Non-mandatory Property - 0..1"@en.

ah:shapeName
	a rdf:Property,	owl:DataProperty;
	rdfs:comment "This properties defines the shape of the arrow. A good pratice is to use the controlled vocabulary AH-ShapeName."@en;
	rdfs:isDefinedBy <http://www.purl.com/ah/vocab/>;
	rdfs:label "ArrowHead - Morphology - BaseDetails-shapeName"@en;
  rdfs:domain ah:BaseShapeDetails;
  rdfs:range ah-vocab:AH-ShapeName;
	vann:usageNote "Optional Property - 0..1"@en.

ah:subtype
	a rdf:Property,	owl:DataProperty;
	rdfs:comment "Presence or absence of fins in the arrowhead base."@en;
	rdfs:isDefinedBy <http://www.purl.com/ah/vocab/>;
	rdfs:label "ArrowHead - Morphology - BaseDetails-subtype."@en;
  rdfs:domain ah:BaseShapeDetails;
	rdfs:range xsd:boolean;
	vann:usageNote "Non-mandatory Property - 0..1"@en.

ah:length
	a rdf:Property,	owl:DataProperty;
	rdfs:comment "Definition of the length of the arrowhead in 'mm'."@en;
	rdfs:isDefinedBy <http://purl.org/dc/terms/>;
	rdfs:label "Arrowhead-Typometry - length"@en;
  rdfs:domain ah:Typometry;
	rdfs:range rdfs:doubleI;
	vann:usageNote "Non-mandatory Property - 0..1"@en.

ah:width
	a rdf:Property,	owl:DataProperty;
	rdfs:comment "Definition of the width of the arrowhead in 'mm'."@en;
	rdfs:isDefinedBy <http://purl.org/dc/terms/>;
	rdfs:label "Arrowhead-Typometry - width"@en;
  rdfs:domain ah:Typometry;
	rdfs:range rdfs:doubleI;
	vann:usageNote "Non-mandatory Property - 0..1"@en.

ah:thickness
	a rdf:Property,	owl:DataProperty;
	rdfs:comment "Definition of the thickness of the arrowhead in 'mm'."@en;
	rdfs:isDefinedBy <http://purl.org/dc/terms/>;
	rdfs:label "Arrowhead-Typometry - thickness"@en;
  rdfs:domain ah:Typometry;
	rdfs:range rdfs:doubleI;
	vann:usageNote "Non-mandatory Property - 0..1"@en.

ah:bodyLenght
	a rdf:Property,	owl:DataProperty;
	rdfs:comment "Definition of the bodyLenght of the arrowhead in 'mm'. Only defined in the case of an arrowhead with a base sapeName 'Triangular', 'Peduncolada' ou 'Losângica'."@en;
	rdfs:isDefinedBy <http://purl.org/dc/terms/>;
	rdfs:label "Arrowhead-Typometry - bodyLenght"@en;
  rdfs:domain ah:Typometry;
	rdfs:range rdfs:doubleI;
	vann:usageNote "Non-mandatory Property - 0..1"@en.


ah:baseLenght
	a rdf:Property,	owl:DataProperty;
	rdfs:comment "Definition of the baseLenght of the arrowhead in 'mm'. Only defined in the case of an arrowhead with a base sapeName 'Triangular', 'Peduncolada' ou 'Losângica'."@en;
	rdfs:isDefinedBy <http://purl.org/dc/terms/>;
	rdfs:label "Arrowhead-Typometry - baseLenght"@en;
  rdfs:domain ah:Typometry;
	rdfs:range rdfs:doubleI;
	vann:usageNote "Non-mandatory Property - 0..1"@en.

  ah:mode
  	a rdf:Property,	owl:DataProperty;
  	rdfs:comment "XXXXXXXXXXXXXXXXXXXXXXXXXXXXXXXXXXXX. A good pratice is to use the COntrolled Vocabulary AH-ChippingMode."@en;
  	rdfs:isDefinedBy <http://www.purl.com/ah/vocab/>;
  	rdfs:label "Arrowhead-Chipping-mode"@en;
    rdfs:domain ah:Chipping;
  	rdfs:range ah-vocab:AH-ChippingMode;
  	vann:usageNote "Non-mandatory Property - 0..1"@en.

ah:amplitude
	a rdf:Property,	owl:DataProperty;
	rdfs:comment "XXXXXXXXXXXXXXXXXXXXXXXXXXXXXXXXXXXX. A good pratice is to use the COntrolled Vocabulary AH-ChippingAmplitude."@en;
	rdfs:isDefinedBy <http://www.purl.com/ah/vocab/>;
	rdfs:label "Arrowhead-Chipping-amplitude"@en;
  rdfs:domain ah:Chipping;
	rdfs:range ah-vocab:AH-ChippingAmplitude;
  vann:usageNote "Non-mandatory Property - 0..1"@en.

ah:direction
	a rdf:Property,	owl:DataProperty;
	rdfs:comment "XXXXXXXXXXXXXXXXXXXXXXXXXXXXXXXXXXXX. A good pratice is to use the COntrolled Vocabulary AH-ChippingDirection."@en;
	rdfs:isDefinedBy <http://www.purl.com/ah/vocab/>;
	rdfs:label "Arrowhead-Chipping-direction"@en;
  rdfs:domain ah:Chipping;
	rdfs:range ah-vocab:AH-ChippingDirection;
  vann:usageNote "Non-mandatory Property - 0..1"@en.

ah:orientation
  	a rdf:Property,	owl:DataProperty;
  	rdfs:comment "XXXXXXXXXXXXXXXXXXXXXXXXXXXXXXXXXXXX. A good pratice is to use the COntrolled Vocabulary AH-ChippingOrientation."@en;
  	rdfs:isDefinedBy <http://www.purl.com/ah/vocab/>;
  	rdfs:label "Arrowhead-Chipping-Orientation"@en;
    rdfs:domain ah:Chipping;
  	rdfs:range ah-vocab:AH-ChippingOrientation;
    vann:usageNote "Non-mandatory Property - 0..1"@en.

ah:delineation
	a rdf:Property,	owl:DataProperty;
	rdfs:comment "XXXXXXXXXXXXXXXXXXXXXXXXXXXXXXXXXXXX. A good pratice is to use the COntrolled Vocabulary AH-ChippingDelineation."@en;
	rdfs:isDefinedBy <http://www.purl.com/ah/vocab/>;
	rdfs:label "Arrowhead-Chipping-delineation"@en;
  rdfs:domain ah:Chipping;
	rdfs:range ah-vocab:AH-ChippingDelineation;
  vann:usageNote "Non-mandatory Property - 0..1"@en.

ah:location
	a rdf:Property,	owl:DataProperty;
	rdfs:comment "XXXXXXXXXXXXXXXXXXXXXXXXXXXXXXXXXXXX. A good pratice is to use the COntrolled Vocabulary AH-ChippingLocation."@en;
	rdfs:isDefinedBy <http://www.purl.com/ah/vocab/>;
	rdfs:label "Arrowhead-Chipping-location"@en;
  rdfs:domain ah:Chipping;
	rdfs:range ah-vocab:AH-ChippingLocation;
  vann:usageNote "Non-mandatory Property - 0..1"@en.

ah:chippingShape
	a rdf:Property,	owl:DataProperty;
	rdfs:comment "XXXXXXXXXXXXXXXXXXXXXXXXXXXXXXXXXXXX. A good pratice is to use the COntrolled Vocabulary AH-ChippingShape."@en;
	rdfs:isDefinedBy <http://www.purl.com/ah/vocab/>;
	rdfs:label "Arrowhead-Chipping-shape"@en;
  rdfs:domain ah:Chipping;
	rdfs:range ah-vocab:AH-ChippingShape;
  vann:usageNote "Non-mandatory Property - 0..1"@en.

#>---------------------------------------------------------<#
#>      THE END END END END END END END END END            <#
#>---------------------------------------------------------<#
