@prefix ah: <http://www.purl.com/ah/ms/ah/> .
@prefix ah-vocab:<http://www.purl.com/ah/ves/>.
@prefix owl: <http://www.w3.org/2002/07/owl#> .
@prefix dct: <http://purl.org/dc/terms/> .
@prefix foaf: <http://xmlns.com/foaf/0.1/> .
@prefix rdfs: <http://www.w3.org/2000/01/rdf-schema#> .
@prefix schema: <http://schema.org/> .
@prefix voaf: <http://labs.mondeca.com/vocab/voaf#> .
@prefix skos: <http://www.w3.org/2004/02/skos/core#> .
@prefix xsd: <http://www.w3.org/2001/XMLSchema#> .
@prefix vann: <http://purl.org/vocab/vann/> .
@prefix dbo:<http://dbpedia.org/ontology/> .
@prefix time:<http://www.w3.org/2006/time#> .
@prefix edm:<http://www.europeana.eu/schemas/edm> .
@prefix crm:<http://www.cidoc-crm.org/cidoc-crm/> .
@prefix crmsci:<https://cidoc-crm.org/extensions/crmsci/> .
@prefix crmarchaeo:<http://www.cidoc-crm.org/extensions/crmarchaeo/> .
@prefix geo:<http://www.w3.org/2003/01/geo/wgs84_pos#> .
@prefix wdrs: <http://www.w3.org/2007/05/powder-s#> .
@prefix rdf: <http://www.w3.org/1999/02/22-rdf-syntax-ns#> .



<http://www.purl.com/ah/ms/ah/> 	a voaf:metadataVoc, owl:Ontology;
  voaf:specializes ah:;
  dct:title "Asset Description Metadata Schema - ArrowHeads' Metadata Scheme"@en;
  rdfs:label "Asset Description Metadata Schema - ArrowHeads' Metadata Scheme"@en;
	dct:abstract "ArowHeads is a profile of Arrowheads Vocabulary, used to describe semantic assets (or just 'Assets'), defined as highly reusable metadata (e.g. xml schemata, generic data models) and reference data (e.g. code lists, taxonomies, dictionaries, vocabularies) that are used for ..............."@en;
	dct:creator [schema:affiliation <http://www.w3.org/data#W3C>;
	  rdfs:seeAlso <http://www.w3.org/TR/rdf-schema/>;
  	foaf:homepage <http://www.w3.org/> ;
  	foaf:name "W3C";
	foaf:maker[foaf:name "XXXXXXXXXXXXXXXXXXXXXXXXX"; foaf:homepage <http://www.w3.org/> ];];
	dct:description """This is the RDF encoding of the data Model for the description of the Chalcolithic and Early/Middle Bronze Age arrowheads .""";
	dct:modified "2024-"^^xsd:date;
	vann:preferredNamespacePrefix "ah";
	vann:preferredNamespaceUri "http://www.purl.com/ah/mes/ah/";
	rdfs:comment "This file specifies the set of RDF classes and properties used in the ArroWheads MAP"@en;
	wdrs:describedby <http://www.yourdomain.com/arrowheads/documentation> .



              #======<>===============================<>=====#
#===========  #------<>-------------------------------<>-----#  ===========#
#===========  #------<>       CLASSES                 <>-----#  ===========#
#===========  #------<>-------------------------------<>-----#	===========#
              #======<>===============================<>=====#

ah:Morphology
	a rdfs:Class;
	rdfs:comment "Morphology of the arrowhead.."@en;
	rdfs:isDefinedBy <http://www.purl.com/ah/ms/ah/>;
	rdfs:label "Morphology"@en.

ah:Typometry
  a rdfs:Class;
  rdfs:comment "Topometry of the arrowhead."@en;
  rdfs:isDefinedBy <http://www.purl.com/ah/ms/ah/>;
  rdfs:label "Typometry"@en.

ah:Chipping
	a rdfs:Class;
	rdfs:comment "Chipping of the arrowhead."@en;
	rdfs:isDefinedBy <http://www.purl.com/ah/ms/ah/>;
  rdfs:label "ArrowHead - Chipping."@en;
	rdfs:label "Shipping"@en.

              #======<>===============================<>=====#
#===========  #------<>-------------------------------<>-----#  ===========#
#===========  #------<>          Properties           <>-----#  ===========#
#===========  #------<>-------------------------------<>-----#	===========#
              #======<>===============================<>=====#

#>-----------------------------------------<#
#>           Object Properties             <#
#>-----------------------------------------<#

ah:foundInCoordinates
	a rdf:Property,	owl:ObjectProperty;
	rdfs:comment "This property points to the GPS coordinates of the location of the arrowhead found."@en;
	rdfs:isDefinedBy <http://www.purl.com/ah/ms/ah/>;
	rdfs:label "ArrowHead - gpslocation"@en;
  rdfs:domain crm:E24_Physical_Man-Made_Thing_Physical_Man-Made_Thing;
	rdfs:range geo:SpatialThing;
	vann:usageNote "Non-mandatory Property - 0..1"@en.

ah:hasMorphology
	a rdf:Property,	owl:ObjectProperty;
	rdfs:comment "This property points to an instance of the definition of the morphology of the arrowhead.."@en;
	rdfs:isDefinedBy <http://www.purl.com/ah/ms/ah/>;
	rdfs:label "ArrowHead - morphology"@en;
  rdfs:domain crm:E24_Physical_Man-Made_Thing_Physical_Man-Made_Thing;
	rdfs:range ah:Morphology;
	vann:usageNote "Non-mandatory Property - 0..1"@en.

ah:hasTypometry
	a rdf:Property,	owl:ObjectProperty;
	dct:identifier "ah:typometry"@en;
	rdfs:comment "This property points to an instance of the definition of the typometry of the Arrowhead."@en;
	rdfs:isDefinedBy <http://www.purl.com/ah/ms/ah/>;
	rdfs:label "ArrowHead - typometry"@en;
  rdfs:domain crm:E24_Physical_Man-Made_Thing_Physical_Man-Made_Thing;
	rdfs:range ah:Typometry;
	vann:usageNote "Non-mandatory Property - 0..1"@en.

ah:hasChipping
  a rdf:Property,	owl:ObjectProperty;
  rdfs:comment "This Property points to an instance of the definition of the chipping of the arrowhead.."@en;
  rdfs:isDefinedBy <http://www.purl.com/ah/ms/ah/>;
  rdfs:label "ArrowHead - has chipping"@en;
  rdfs:domain crm:E24_Physical_Man-Made_Thing_Physical_Man-Made_Thing;
  rdfs:range ah:Chipping;
  vann:usageNote "Non mandatory Property - 0..1"@en.


#>-----------------------------------------<#
#>           Data Properties             <#
#>-----------------------------------------<#

ah:shape
	a rdf:Property,	owl:DataProperty;
	rdfs:comment "This property records the shape of the arrowhead. A good practice is to use the controlled vocabulary for AH-Shape."@en;
	rdfs:isDefinedBy <http://www.purl.com/ah/ms/ah/>;
	rdfs:label "ArrowHead - shape"@en;
        rdfs:domain crm:E24_Physical_Man-Made_Thing;
	rdfs:range ah-vocab:ah-shape;
	vann:usageNote "Non-mandatory Property - 0..1"@en.

ah:variant
  	a rdf:Property,	owl:DataProperty;
  	rdfs:comment "Thickness Index. This is calculated by dividing the maximum width by the maximum thickness. The arrowhead is characterised as 'Blunt' when the index is equal to or greater than 8; 'Raised' when less than 8 and greater than  A good practice is to use the Controlled Vocabulary AH-Variant."@en;
        rdfs:comment "Indice de Espessura. Calcula-se o valor da divisão largura máxima e espessura máxima. A ponta de seta é  caracterizada como 'Abatida' quando o índice é igual ou superior a 8; 'Alteada' quando inferior a 8 e superior a 4, e 'Espessa' quando inferior a 4. Usar o vocabulário controlado Ah-Variant"@pt;
  	rdfs:isDefinedBy <http://www.purl.com/ah/ms/ah/>;
  	rdfs:label "ArrowHead - arrowHeadVariant"@en;
        rdfs:domain crm:E24_Physical_Man-Made_Thing;
  	rdfs:range ah-vocab:ah-variant;
  	vann:usageNote "Optional Property - 0..1"@en.

ah:point
	a rdf:Property,	owl:DataProperty;
	rdfs:comment "Definition of the tip of the arrowhead. Sharp=True;Fractured=False."@en;
	 rdfs:comment "Definição da ponta da ponta de seta. Sharp=True;Fractured=False."@pt;
	rdfs:isDefinedBy <http://purl.org/dc/terms/>;
	rdfs:label "Arrowhead-Morphology - point. Sharp=True;Fractured=False"@en;
  rdfs:label "Arrowhead-Morphology - point. Piquant=True;Não Piquant=False"@pt;
 rdfs:domain ah:Morphology;
	rdfs:range xsd:boolean;
	vann:usageNote "Non-mandatory Property - 0..1"@en .

ah:body
	a rdf:Property,	owl:DataProperty;
        rdfs:comment "THis property is used to define the simmetry of the body of the arrowhead presents. Symmetrical=True; Non-symmetrical=False"@en;
	  rdfs:comment "Esta propriedade define a simetria da base da ponta de seta. Symmetrical=True; Non-symmetrical=False";
	rdfs:isDefinedBy <http://www.purl.com/ah/ms/ah/>;
	rdfs:label "Arrowhead-Morphology - body. Symmetrical=True; Non-symmetrical=False. "@en;
	rdfs:label "Arrowhead-Morphology - body. Symmetrical=True; Non-symmetrical=False. "@pt;
        rdfs:domain ah:Morphology;
	rdfs:range xsd:boolean;
	vann:usageNote "Non-mandatory Property - 0..1"@en.

ah:base
	a rdf:Property,	owl:DataProperty;
	rdfs:comment "This properties defines the base of the arrowhead. A good pratice is to use the controlled vocabulary AH-Base."@en;
	  rdfs:comment "Esta propriedade é usada para categorizar a base da ponta de seta. Usar o vocabulário controlado AH-Base."@pt;
	rdfs:isDefinedBy <http://www.purl.com/ah/ms/ah/>;
	rdfs:label "ArrowHead - Morphology - Base. A good pratice is to use the Controlled Vocabulary AH-Base. "@en;
	rdfs:label "ArrowHead - Morphology - Base. Uma boa prática é usar o vocabulário controlado AH-Base. "@pt;
	rdfs:domain ah:Morphology;
	rdfs:range ah-vocab:AH-Base;
	vann:usageNote "Optional Property - 0..1"@en.

  ah:mode
  	a rdf:Property,	owl:DataProperty;
  	rdfs:comment "Type of retouching incidence, defines the angle formed by the retouching line and the chipping surface. A good pratice is to use the Controlled Vocabulary AH-ChippingMode."@en;
        rdfs:comment "Tipo de incidência do retoque, define o ângulo formado pela linha de retoque e a superfície de lascagem. Usar o vocabulário controlado AH-Mode."@pt;
  	rdfs:isDefinedBy <http://www.purl.com/ah/ms/ah/>;
  	rdfs:label "Arrowhead-Chipping-mode"@en;
        rdfs:domain ah:Chipping;
  	rdfs:range ah-vocab:AH-ChippingMode;
  	vann:usageNote "Non-mandatory Property - 0..1"@en.

ah:amplitude
	a rdf:Property,	owl:DataProperty;
	rdfs:comment "Retouching extension, Marginal=True;Deep=False."@en;
        rdfs:comment "Extensão do retoque, Marginal=True;Profundo=False."@pt;
	rdfs:isDefinedBy <http://www.purl.com/ah/ms/ah/>;
	rdfs:label "Arrowhead-Chipping-amplitude"@en;
        rdfs:domain ah:Chipping;
	rdfs:range xsd:boolean;
        vann:usageNote "Non-mandatory Property - 0..1"@en.

ah:direction
	a rdf:Property,	owl:DataProperty;
	rdfs:comment "It results from the position in which the chip or blade is placed to be retouched. A good pratice is to use the Controlled Vocabulary AH-ChippingDirection."@en;
        rdfs:comment "Resulta da posição em que é colocada a lasca ou lamina para ser retocada. Usar o vocabulário controlado AH-ChippingDirection."@pt;
        rdfs:isDefinedBy <http://www.purl.com/ah/ms/ah/>;
	rdfs:label "Arrowhead-Chipping-direction"@en;
        rdfs:domain ah:Chipping;
	rdfs:range ah-vocab:AH-ChippingDirection;
        vann:usageNote "Non-mandatory Property - 0..1"@en.

ah:orientation
  	a rdf:Property,	owl:DataProperty;
  	rdfs:comment "Angle between the original axis of the part and the line formed by the retouching, Lateral=True;Transverse=False."@en;
    	rdfs:comment "Ângulo entre o eixo primitivo da peça e a linha formada pelo retoque, Lateral=True;Transversal=False."@pt;
  	rdfs:isDefinedBy <http://www.purl.com/ah/ms/ah/>;
  	rdfs:label "Arrowhead-Chipping-Orientation"@en;
 	rdfs:domain ah:Chipping;
  	rdfs:range xsd:boolean;
    	vann:usageNote "Non-mandatory Property - 0..1"@en.

ah:delineation
	a rdf:Property,	owl:DataProperty;
	rdfs:comment "The retouching gives the margins a shape.. A good pratice is to use the Controlled Vocabulary AH-ChippingDelineation."@en;
 	rdfs:comment "Ângulo entre o eixo primitivo da peça e a linha formada pelo retoque. Usar o vocabulário controlado AH-ChippingOrientation."@pt;
	rdfs:isDefinedBy <http://www.purl.com/ah/ms/ah/>;
	rdfs:label "Arrowhead-Chipping-delineation"@en;
  	rdfs:domain ah:Chipping;
	rdfs:range ah-vocab:AH-ChippingDelineation;
  	vann:usageNote "Non-mandatory Property - 0..1"@en.

ah:chippinglocation-Side
	a rdf:Property,	owl:DataProperty;
	rdfs:comment "The retouching can occupy a position to the left or right of the axis of symmetry and, depending on the axis perpendicular to it, the retouching can be distal, medial or proximal. . A good pratice is to use the COntrolled Vocabulary AH-ChippingLocation."@en;
  	rdfs:comment "Ângulo entre o eixo primitivo da peça e a linha formada pelo retoque. Usar o vocabulário controlado AH-ChippingLocation."@pt;
	rdfs:isDefinedBy <http://www.purl.com/ah/ms/ah/>;
	rdfs:label "Arrowhead-Chipping Location-lateral"@en;
	rdfs:domain ah:Chipping;
	rdfs:range ah-vocab:AH-ChippingLocation;
	vann:usageNote "Non-mandatory Property - 0..3"@en.

ah:chippinglocation-Transversal
  	a rdf:Property,	owl:DataProperty;
  	rdfs:comment "The retouching can be distal or proximal and, depending on the edge where it is located, it can occupy a left, right or median position. A good pratice is to use the COntrolled Vocabulary AH-ChippingLocation."@en;
	rdfs:comment "O retoque pode ser distal ou próximal e em função do bordo onde se situa, pode ocupar uma posição à esquerda, à direita, ou mediana. Usar o vocabulário controlado AH-ChippingLocation."@pt;
  	rdfs:isDefinedBy <http://www.purl.com/ah/ms/ah/>;
  	rdfs:label "Arrowhead-Chipping Location-Transversal"@en;
	rdfs:domain ah:Chipping;
  	rdfs:range ah-vocab:AH-ChippingLocation;
  	vann:usageNote "Non-mandatory Property - 0..3"@en.

ah:chippingShape
	a rdf:Property,	owl:DataProperty;
	rdfs:comment "Line defined by the edge. A good pratice is to use the Controlled Vocabulary AH-ChippingShape."@en;
	rdfs:comment "Linha definida pelo bordo. Usar o vocabulário controlado AH-ChippingShape."@pt;
	rdfs:isDefinedBy <http://www.purl.com/ah/ms/ah/>;
	rdfs:label "Arrowhead-Chipping-shape"@en;
  	rdfs:domain ah:Chipping;
	rdfs:range ah-vocab:AH-ChippingShape;
  	vann:usageNote "Non-mandatory Property - 0..1"@en.

#>---------------------------------------------------------<#
#>      THE END END END END END END END END END            <#
#>---------------------------------------------------------<#
